DynamoDbEncryptionMiddlewareInternal/runtimes/java/src/main/smithy-generated/software/amazon/cryptography/dynamoDbEncryption/model/Lower.java
@@ -1,0 +1,33 @@
+// Copyright Amazon.com Inc. or its affiliates. All Rights Reserved.
+// SPDX-License-Identifier: Apache-2.0
+// Do not modify this file. This file is machine generated, and any changes to it will be overwritten.
+package software.amazon.cryptography.dynamoDbEncryption.model;
+
+public class Lower {
+  protected Lower(BuilderImpl builder) {
+  }
+
+  public Builder toBuilder() {
+    return new BuilderImpl(this);
+  }
+
+  public static Builder builder() {
+    return new BuilderImpl();
+  }
+
+  public interface Builder {
+    Lower build();
+  }
+
+  static class BuilderImpl implements Builder {
+    protected BuilderImpl() {
+    }
+
+    protected BuilderImpl(Lower model) {
+    }
+
+    public Lower build() {
+      return new Lower(this);
+    }
+  }
+}
